---
title: Coupled Perturbed Self-Consistent Field Method
author: HXu
date: 2023-06-16
category: notes
layout: post
---

## Motivation

To evaluate second-order properties, we need the perturbed AO density matrices. For example,
for the paramagnetic contribution to the NMR shielding tensor, we need:

$$
\begin{align}
  ^{\text{SCF}}_{\text{para}}\sigma _{ji}^{N} =& \sum_{\mu \nu}\frac{\partial D _{\mu \nu}^{\text{SCF}}}{\partial B _{i}}\frac{\partial h _{\mu \nu}}{\partial m _{N j}} \\
\end{align}
$$

By parameterizing the perturbed MO coefficients with unitary matrix $\mathbf{U}$ :

$$
\begin{align}
  \pdv{C _{\mu p}}{\mathbf{B}} = \sum_{r}C _{\mu r}\pdv{U _{rp}}{\mathbf{B}}
\end{align} 
$$

we can then express the perturbed AO densities as:

$$
\begin{align}
  \pdv{D _{\mu \nu}^{\text{SCF}}}{\mathbf{B}} =& \pdv{\mathbf{B}}\sum_{i}C _{\mu i}^{*}C _{\nu i}
  = \sum_{ir}\left\{\pdv{U _{ri}^{*}}{\mathbf{B}}C _{\mu r}^{*}C _{\nu i}+C _{\mu i}^{*}C _{\nu r}\pdv{U _{ri}}{\mathbf{B}}\right\} \\
\end{align}
$$

We denote $\pdv{U _{pq}}{\mathbf{B}}$ simply as $U _{pq}^{\mathbf{B}}$ , and these coefficients are determined by solving the CPSCF equations.

## CPSCF Equations

The CPSCF equations are derived from two conditions which need to be fullfilled by
the MO coefficients, in the presence of any types external perturbation.
These are the Orthonormality Condition, and the Brillouin Condition:

$$
\begin{align}
  S _{pq} = \delta _{pq} && f _{ai} = 0
\end{align}
$$

Differentiating these conditions w.r.t the perturbation parameter $\lambda$ gives us the constraints for the CPSCF coefficients $U _{pq}^{\lambda}$ :

$$
\begin{align}
  \pdv{S _{pq}}{\lambda} = 0 && \pdv{f _{ai}}{\lambda} = 0
\end{align}
$$

Evaluating the first condition by expanding the overlap matrix:

$$
\begin{align}
  \pdv{S _{pq}}{\lambda} =& \pdv{\lambda}\sum_{\mu \nu}C _{\mu p}^{*}S _{\mu \nu}C _{\nu q} \nonumber \\
  0=& S _{pq}^{(\lambda)} + \sum_{\mu \nu}\sum_{r}\left\{\pdv{U _{rp}^{*}}{\lambda}C _{\mu r}^{*} S _{\mu \nu} C _{\nu q}
  + C _{\mu p}^{*}S _{\mu \nu}C _{\nu r}\pdv{U _{rq}}{\lambda}\right\} \nonumber \\
  0=& S _{pq}^{(\lambda)} + \sum_{r}\left\{U _{rp}^{*}S _{rq} + U _{rq}S _{pr}\right\}
\end{align}
$$

which leads to:

$$
\begin{align}
  0=& U _{qp}^{\lambda*} + S _{pq}^{(\lambda)} + U _{pq}^{\lambda}
\end{align}
$$

in which $S ^{(\lambda)}_{pq}$ represents the derivative of AO overlap matrix rotated into MO basis.

The second condition gives:

$$
\begin{align}
  \pdv{f _{ai}}{\lambda} =& \pdv{\lambda}\left\{\sum_{\mu \nu}C _{\mu a}^{*}h _{\mu \nu}C _{\nu i}
  +\sum_{\mu \nu \rho \sigma}\sum_{m}C _{\mu a}^{*}C _{\nu m}\langle \mu \nu||\rho \sigma\rangle C _{\rho i}C _{\sigma m}\right\} \nonumber \\
  0=& \sum_{\mu \nu} C _{\mu a}\pdv{h _{\mu \nu}}{\lambda }C _{\nu i} + \sum_{\mu \nu \rho \sigma}\sum_{m}C _{\mu a}^{*}C _{\nu m}\pdv{\langle \mu \nu ||\rho \sigma\rangle}{\lambda}C _{\rho i}C _{\sigma m} \nonumber \\
   &+\sum_{\mu \nu}h _{\mu \nu}\sum_{r}\left\{\pdv{U _{ra}^{*}}{\lambda}C _{\mu r}^{*}C _{\nu i} + C _{\mu a}^{*}C _{\nu r}\pdv{U _{ri}}{\lambda}\right\} \nonumber \\
   &+ \sum_{\mu \nu \rho \sigma}\sum_{m}\langle \mu \nu||\sigma \rho\rangle \left\{\pdv{U _{ra}^{*}}{\lambda}C _{\mu r}^{*} C _{\nu m}^{*} C _{\rho i}C _{\sigma m}
   + \pdv{U _{rm}^{*}}{\lambda}C _{\mu a}^{*}C _{\nu r}^{*}C _{\rho i}C _{\sigma m}\right\} \nonumber \\
   & + \sum_{\mu \nu \rho \sigma}\sum_{m}\langle \mu \nu||\sigma \rho \rangle \left\{C _{\mu a}^{*}C _{\nu m}^{*}C _{\rho r}C _{\sigma m}\pdv{U _{ri}}{\lambda}
   + C _{\mu a}^{*}C _{\nu m}^{*}C _{\rho i}C _{\sigma r}\pdv{U _{rm}}{\lambda}\right\} \nonumber \\
  0=& h _{ai}^{(\lambda)} + \sum_{m}\langle am||im\rangle ^{(\lambda)} + \sum_{r}h _{ri}U _{ra}^{\lambda*} + \sum_{r}h _{ar}U _{ri}^{\lambda} \nonumber \\
  &+ \sum_{mr} \left\{\langle rm||im\rangle U _{ra}^{\lambda *} + \langle ar||im\rangle U _{rm}^{\lambda*} + \langle am||rm\rangle U _{ri}^{\lambda} + \langle am||ir\rangle U _{rm}^{\lambda}\right\} \nonumber \\
  0=&h _{ai}^{(\lambda)} + \sum_{m}\langle am||im\rangle ^{(\lambda)} + \sum_{r}f _{ri}U _{ra}^{\lambda*} + \sum_{r}f _{ar}U _{ri}^{\lambda} \nonumber \\
  &+ \sum_{mr}\left\{\langle ar||im\rangle U _{rm}^{\lambda*} + \langle am||ir\rangle U _{rm}^{\lambda}\right\} \nonumber \\
  0=&h _{ai}^{(\lambda)} + \sum_{m}\langle am||im\rangle ^{(\lambda)} + \sum_{r}f _{ii}\delta _{ri} U _{ra}^{\lambda*} + \sum_{r}f _{aa}\delta _{ar} U _{ri}^{\lambda} \nonumber \\
  &+ \sum_{me}\left\{\langle ae||im\rangle U _{em}^{\lambda*}+\langle am||ie\rangle U _{em}^{\lambda}\right\} + \sum_{mn}\left\{\langle an||im\rangle U _{nm}^{\lambda *}+\langle am||in\rangle U _{nm}^{\lambda}\right\}
\end{align}
$$

Using the Orthonormality Condition, the last term could be re-written as:

$$
\begin{align}
  \sum_{mn}\left\{\langle an||im\rangle U _{nm}^{\lambda*} + \langle an||im\rangle U _{mn}^{\lambda} \right\}= -\sum_{mn}\langle an||im\rangle S _{mn}^{(\lambda)}
\end{align}
$$

and the $f _{ii}$ term as:

$$
\begin{align}
  f _{ii}U _{ia}^{\lambda*} = f _{ii}(-U _{ai}^{\lambda}-S _{ai}^{(\lambda)})
\end{align}
$$

By collecting the $U$-dependent terms on the LHS, the final CPSCF equation could be expressed as:

$$
\begin{align}
  (f _{aa}-f _{ii})U _{ai}^{\lambda} + \sum_{me}\left\{\langle ae||im\rangle U _{em}^{\lambda *} + \langle am||ie\rangle U _{em}^{\lambda}\right\} = -B _{ai}^{\lambda}
\end{align}
$$

with

$$
\begin{align}
  B _{ai}^{\lambda} = h _{ai}^{(\lambda)} + \sum_{m}\langle am||im\rangle ^{(\lambda)}-S _{ai}^{(\lambda)}f _{ii}-\sum_{mn}S _{mn}^{(\lambda)}\langle an||im\rangle
\end{align}
$$

Up until this point we have not assumed anything about the nature of the perturbation, which means the result is general regarding the type of perturbation.  

We could further divide the equations into two cases, for real and imaginary perturbations respectively.
We can investigate each case by writing the CPSCF coefficient into complex form and inspect the derivatives correspondingly:

$$
\begin{align}
  \mathbf{U} ^{\lambda} =& \mathfrak{Re}\{\mathbf{U}^{\lambda}\} + \mathrm{i}\mathfrak{Im}\{\mathbf{U}^{\lambda}\}
\end{align}
$$

For purely real and purely imaginary perturbations, e.g. electric and magnetic, respectively, they would contain only the real $(\mathfrak{Re})$ or imaginary $(\mathfrak{Im})$ part.
Therefore:

$$
\begin{align}
  \mathbf{U}^{\mathbf{E}*} = \mathbf{U}^{\mathbf{E}} && \mathbf{U}^{\mathbf{B}*} = -\mathbf{U}^{\mathbf{B}}
\end{align}
$$

Meanwhile, the RHS would be purely real or purely imaginary, in respective case:

$$
\begin{align}
  B _{ai}^{\mathbf{E}} \in \mathbb{R} && B _{ai}^{\mathbf{B}} \in \mathbb{Im}
\end{align}
$$

This comes from the real/imaginary nature of the integral derivatives in each case.  

Therefore, the CPSCF equations subject to electric perturbations are:

$$
\begin{align}
  (f _{aa} - f _{ii})U _{ai}^{\mathbf{E}} + \sum_{me}U _{em}^{\mathbf{E}}\left\{\langle am||ie\rangle + \langle ae||im\rangle\right\} = -B _{ai}^{\mathbf{E}}
\end{align}
$$

and the magnetic ones:

$$
\begin{align}
  (f _{aa} - f _{ii})U _{ai}^{\mathbf{B}} + \sum_{me}U _{em}^{\mathbf{B}}\left\{\langle am||ie\rangle - \langle ae||im\rangle\right\} = -B _{ai}^{\mathbf{B}}
\end{align}
$$

with

$$
\begin{align}
  B _{ai}^{\lambda} = h _{ai}^{(\lambda)} + \sum_{m}\langle am||im\rangle ^{(\lambda)}-S _{ai}^{(\lambda)}f _{ii}-\sum_{mn}S _{mn}^{(\lambda)}\langle an||im\rangle
\end{align}
$$

For computational convenience, this could also be written in matrix form, by combining $ai$ into a single index:

$$
\begin{align}
  \mathbf{A}\mathbf{U}^{\lambda} = -\mathbf{B}^{\lambda} && \Leftrightarrow && \sum_{em}A _{ai,em}U ^{\lambda}_{em} = -B _{ai}^{\lambda}
\end{align}
$$

and the matrix $\mathbf{A}$ differs in magnetic and electric cases.  

<br/>

For occupied-occupied block and virtual-virtual block, the U coefficients could be chosen arbitrarily as long as the derivative orthonormality condition is fullfilled.
Most conveniently, we choose:

$$
\begin{align}
  U _{ij}^{\lambda} = -\frac{1}{2}S _{ij}^{(\lambda)} = U _{ji}^{\lambda*} && U _{ab}^{\lambda} = -\frac{1}{2}S _{ab}^{(\lambda)} = U _{ba}^{\lambda *}
\end{align}
$$